{
 "cells": [
  {
   "cell_type": "markdown",
   "metadata": {},
   "source": [
    "### 1.10 Exercises"
   ]
  },
  {
   "cell_type": "markdown",
   "metadata": {},
   "source": [
    "**Exercise 1.1**.  Let $A_1$ and $A_2$ be arbitrary events and show that $\\text{Pr}\\{A_1 \\cup A_2\\} + \\text{Pr}\\{A_1 A_2\\} = \\text{Pr}\\{A_1\\} + \\text{Pr}\\{A_2\\}$.  Explain which parts of the sample space are being double counted on both sides of this equation and which parts are being counted once."
   ]
  },
  {
   "cell_type": "markdown",
   "metadata": {},
   "source": [
    "**Solution**.  Consider the disjoint events $A_1 - A_2, A_2 - A_1, A_1 A_2$, where $X - Y = \\{ \\omega : \\omega \\in X \\text{ and not } \\omega \\in Y \\}$.  \n",
    "\n",
    "By construction these events are disjoint: any event $\\omega$ either:\n",
    "\n",
    "- belongs to $A_1$ but not $A_2$, in which case $\\omega \\in A_1 - A_2$ but it does not belong to $A_2 - A_1$ or $A_1 A_2$;\n",
    "- belongs to $A_2$ but not $A_1$, in which case $\\omega \\in A_2 - A_1$ but it does not belong to $A_1 - A_2$ or $A_1 A_2$;\n",
    "- belongs to both $A_1$ and $A_2$, in which case $\\omega \\in A_1 A_2$ but it does not belong to $A_1 - A_2$ or $A_2 - A_1$;\n",
    "- does not belong to $A_1$ or $A_2$, in which case it does not belong to any of $A_1 - A_2, A_2 - A_1, A_1 A_2$.\n",
    "\n",
    "Also note that:\n",
    "\n",
    "- $(A_1 - A_2) \\cup A_1 A_2 = A_1$, since any event that belongs to $A_1$ either belongs to $A_2$ (in which case it belongs to $A_1 A_2$) or not (in which case it belongs to $A_1 - A_2$).\n",
    "- $(A_2 - A_1) \\cup A_1 A_2 = A_2$, by a similar argument.\n",
    "- $(A_1 - A_2) \\cup (A_2 - A_1) \\cup A_1 A_2 = A_1 \\cup A_2$, by applying the union over the previous two statements.\n",
    "\n",
    "By the third axiom of probability (using the finite version -- add infinitely many empty to get an infinite sequence) we get:\n",
    "\n",
    "1.  $\\text{Pr}\\{A_1 - A_2\\} + \\text{Pr}\\{ A_1 A_2 \\} = \\text{Pr}\\{A_1\\} $\n",
    "2.  $\\text{Pr}\\{A_2 - A_1\\} + \\text{Pr}\\{ A_1 A_2 \\} = \\text{Pr}\\{A_2\\} $\n",
    "3.  $\\text{Pr}\\{A_1 \\cup A_2 \\} = \\text{Pr}\\{A_1 - A_2\\} + \\text{Pr}\\{ A_2 - A_1 \\} + \\text{Pr}\\{ A_1 A_2 \\}$\n",
    "\n",
    "Adding these three statements, we get the desired result,\n",
    "\n",
    "$$\\text{Pr}\\{A_1 \\cup A_2\\} + \\text{Pr}\\{A_1 A_2\\} = \\text{Pr}\\{A_1\\} + \\text{Pr}\\{A_2\\}$$\n",
    "\n",
    "Note that:\n",
    "\n",
    "- If $\\omega \\in A_1$ and $\\omega \\in A_2$, it is counted twice in each side of the equation -- once in $\\text{Pr}\\{A_1 \\cup A_2\\}$, once in $\\text{Pr}\\{A_1 A_2\\}$, once in $\\text{Pr}\\{A_1\\}$ and once in $\\text{Pr}\\{A_2\\}$.\n",
    "- If $\\omega \\in A_1$ but $\\text{not } \\omega \\in A_2$, it is counted once in each side of the equation -- once in $\\text{Pr}\\{A_1 \\cup A_2\\}$ and once in $\\text{Pr}\\{A_1\\}$.\n",
    "- If $\\omega \\in A_2$ but $\\text{not } \\omega \\in A_1$, it is counted once in each side of the equation -- once in $\\text{Pr}\\{A_1 \\cup A_2\\}$ and once in $\\text{Pr}\\{A_2\\}$.\n",
    "- If $\\text{not } \\omega \\in A_1$ and $\\text{not } \\omega \\in A_2$, it is counted zero times in each side of the equation."
   ]
  },
  {
   "cell_type": "markdown",
   "metadata": {},
   "source": [
    "**Exercise 1.2**.  This exercise derives the probability of an arbitrary (non-disjoint) union of events, derives the union bound, and derives some useful limit expressions.\n",
    "\n",
    "**(a)** For two arbitrary events $A_1$ and $A_2$, show that\n",
    "\n",
    "$$ A_1 \\cup A_2 = A_1 \\cup (A_2 - A_1) \\quad \\text{where } A_2 - A_1 = A_2 A_1^c$$\n",
    "\n",
    "Show that $A_1$ and $A_2 - A_1$ are disjoint.  Hint:  Venn diagrams were invented to help understand expressions like these.\n",
    "\n",
    "**(b)** For an arbitrary sequence of events, $\\{A_n : n \\geq 1\\}$, let $B_1 = A_1$ and for each $n \\geq 2$ define $B_n = A_n - \\cup_{m=1}^{n - 1} A_m$.  Show that $B_1, B_2, \\dots$ are disjoint events and show that for each $n \\geq 2$, $\\cup_{m=1}^n A_m = \\cup_{m=1}^n B_m$.  Hint: Use induction.\n",
    "\n",
    "**(c)** Show that\n",
    "\n",
    "$$ \\text{Pr}\\left\\{ \\cup_{n=1}^\\infty A_n \\right\\} = \\text{Pr}\\left\\{ \\cup_{n=1}^\\infty B_n \\right\\} = \\sum_{n=1}^\\infty \\text{Pr} \\left\\{ B_n \\right\\} $$\n",
    "\n",
    "Hint: Use the axioms of probability for the second equality.\n",
    "\n",
    "**(d)** Show that for each $n$, $\\text{Pr}\\left\\{ B_n \\right\\} \\leq \\text{Pr} \\left\\{ A_n \\right\\}$.  Use this to show that\n",
    "\n",
    "$$ \\text{Pr}\\left\\{ \\cup_{n=1}^\\infty A_n \\right\\} \\leq \\sum_{n=1}^\\infty \\text{Pr} \\left\\{ A_n \\right\\} $$\n",
    "\n",
    "**(e)** Show that $\\text{Pr}\\left\\{ \\cup_{n=1}^\\infty A_n \\right\\} = \\lim_{m \\rightarrow \\infty} \\text{Pr} \\left\\{ \\cup_{n=1}^m A_n \\right\\}$.  Hint: Combine (c) and (b).  Note that this says that the probability of a limit of unions is equal to the limit of probabilities.  This might well appear to be obvious without a proof, but you will see situations later where similar appearing interchanges cannot be made.\n",
    "\n",
    "**(f)** Show that $\\text{Pr}\\left\\{ \\cap_{n=1}^\\infty A_n \\right\\} = \\lim_{n \\rightarrow \\infty} \\text{Pr}\\left\\{ \\cap_{i=1}^n A_i \\right\\}$.  Hint: Remember De Morgan's equalities."
   ]
  },
  {
   "cell_type": "markdown",
   "metadata": {},
   "source": [
    "**Solution**."
   ]
  },
  {
   "cell_type": "markdown",
   "metadata": {},
   "source": [
    "**(a)**  We have:\n",
    "\n",
    "$$ \n",
    "\\begin{align}\n",
    "&\\omega \\in A_1 \\cup A_2 \\\\\n",
    "&\\Longleftrightarrow (\\omega \\in A_1) \\lor (\\omega \\in A_2) \\\\\n",
    "&\\Longleftrightarrow (\\omega \\in A_1) \\lor (\\omega \\in A_2 \\land \\neg(\\omega \\in A_1)) \\\\\n",
    "&\\Longleftrightarrow (\\omega \\in A_1) \\lor (\\omega \\in (A_2 - A_1)) \\\\\n",
    "&\\Longleftrightarrow \\omega \\in A_1 \\cup (A_2 - A_1) \\\\\n",
    "\\end{align}\n",
    "$$\n",
    "\n",
    "where we can explicitly verify the third step with a truth table:\n",
    "\n",
    "$$\n",
    "\\begin{array}{cc|c|c}\n",
    "\\omega \\in A_1 & \\omega \\in A_2 & (\\omega \\in A_1) \\lor (\\omega \\in A_2) & (\\omega \\in A_1) \\lor (\\omega \\in A_2 \\land \\neg(\\omega \\in A_1)) \\\\\n",
    "\\hline\n",
    "T & T & T & T \\\\\n",
    "T & F & T & T \\\\\n",
    "F & T & T & T \\\\\n",
    "F & F & F & F\n",
    "\\end{array}\n",
    "$$\n",
    "\n",
    "Since the sets $A_1 \\cup A_2$ and $A_1 \\cup (A_2 - A_1)$ have equivalent statements determining whether a granular event $\\omega$ belongs to them, they are equal,\n",
    "\n",
    "$$ A_1 \\cup A_2 = A_1 \\cup (A_2 - A_1) $$"
   ]
  },
  {
   "cell_type": "markdown",
   "metadata": {},
   "source": [
    "**(b)**  Let's use induction.\n",
    "\n",
    "For the base case, $n = 2$, we have $B_2 = A_2 - A_1$.  \n",
    "- Note that $B_1 = A_1$ and $B_2$ are disjoint events by construction: every element from $A_1$ is explicitly excluded from $B_2$.  \n",
    "- Also note that $A_1 \\cup A_2 = B_1 \\cup B_2$, since $B_1 \\cup B_2 = A_1 \\cup (A_2 - A_1)$, and this is the result proved in (a).\n",
    "\n",
    "For the induction step, assume the result is true for $n$.  \n",
    "- Since $B_{n + 1} = A_n - \\cup_{i=1}^n A_m$, any element belonging to $B_{n+1}$ will not belong to any of the $A_m$ for $1 \\leq m \\leq n$ by construction, and since from the previous step $\\cup_{m=1}^n A_m = \\cup_{m=1}^n B_m$, it will also not belong to any $B_m$, $1 \\leq m \\leq n$.  Therefore there is no overlap between $B_{n + 1}$ and $B_m$, and the $B_i$'s are disjoint.\n",
    "- Finally, note that, from applying (a) on sets $A_{n + 1}$ and $\\cup_{m=1}^n A_m$,\n",
    "\n",
    "$$ \n",
    "\\begin{align}\n",
    "A_{n + 1} \\cup \\left( \\cup_{m=1}^n A_m \\right) &= \\left( \\cup_{m=1}^n A_m \\right) \\cup \\left(A_{n+1} - \\left( \\cup_{m=1}^n A_m \\right)  \\right) \\\\ \n",
    "A_{n + 1} \\cup \\left( \\cup_{m=1}^n A_m \\right) &= \\left( \\cup_{m=1}^n B_m \\right) \\cup B_{n+1} \\\\\n",
    "\\cup_{m=1}^{n+1} A_m &= \\cup_{m=1}^{n+1} B_m \n",
    "\\end{align}\n",
    "$$"
   ]
  },
  {
   "cell_type": "markdown",
   "metadata": {},
   "source": [
    "**(c)**  The result follows from the third axiom of inequality, since all of the $B_i$'s are disjoint by (b)."
   ]
  },
  {
   "cell_type": "markdown",
   "metadata": {},
   "source": [
    "**(d)**  We have $B_n = A_n - \\cup_{m=1}^{n - 1} A_m = A_n - \\cup_{m=1}^{n - 1} B_m$, and so uniting both sides to $\\cup_{m=1}^{n - 1} B_m$ we get $\\cup_{m=1}^{n} B_m = A_n$.  Since the $B_i$'s are disjoint, by the third axiom of probability we have\n",
    "\n",
    "$$ \\text{Pr}\\left\\{A_n\\right\\} = \\sum_{m=1}^n \\text{Pr}\\left\\{ B_m \\right\\} = \\sum_{m=1}^{n - 1} \\text{Pr}\\left\\{ B_m \\right\\} + \\text{Pr}\\left\\{B_n\\right\\}$$\n",
    "\n",
    "and, since for the first axiom of probability,  $\\text{Pr} \\left\\{ B_m \\right\\} \\geq 0$ for $1 \\leq m \\leq n - 1$, we get\n",
    "\n",
    "$$ \\text{Pr}\\left\\{A_n\\right\\} \\geq \\text{Pr}\\left\\{B_n\\right\\} $$\n",
    "\n",
    "Finally, using this inequality for each $n$, and from (b), we have\n",
    "\n",
    "$$ \\text{Pr}\\left\\{ \\cup_{n=1}^\\infty A_n \\right\\} \n",
    "= \\text{Pr}\\left\\{ \\cup_{n=1}^\\infty B_n \\right\\} \n",
    "= \\sum_{n=1}^\\infty \\text{Pr} \\left \\{ B_n \\right\\}\n",
    "\\leq \\sum_{n=1}^\\infty \\text{Pr} \\left\\{ A_n \\right\\} $$\n"
   ]
  },
  {
   "cell_type": "markdown",
   "metadata": {},
   "source": [
    "**(e)**  The result from (c) states that\n",
    "\n",
    "$$ \\text{Pr}\\left\\{ \\cup_{n=1}^\\infty A_n \\right\\} = \\text{Pr}\\left\\{ \\cup_{n=1}^\\infty B_n \\right\\} = \\sum_{n=1}^\\infty \\text{Pr} \\left\\{ B_n \\right\\} $$\n",
    "\n",
    "In particular, we can consider a different sequence of sets, $A'_1, A'_2, \\dots$ and $B'_1, B'_2, \\dots$, where\n",
    "\n",
    "$$\n",
    "A'_k = \\begin{cases}\n",
    "A_k &\\text{if } k \\leq n \\\\\n",
    "A_n &\\text{if } k > n\n",
    "\\end{cases}\n",
    "\\quad \\text{and} \\quad\n",
    "B'_k = \\begin{cases}\n",
    "B_k &\\text{if } k \\leq n \\\\\n",
    "\\varnothing &\\text{if } k >n\n",
    "\\end{cases}\n",
    "$$\n",
    "\n",
    "Since the previous results also apply to these sequences of sets, the finite version of the result is also valid for every $n$,\n",
    "\n",
    "$$ \\text{Pr}\\left\\{ \\cup_{m=1}^n A_m \\right\\} = \\text{Pr}\\left\\{ \\cup_{m=1}^n B_m \\right\\} = \\sum_{m=1}^n \\text{Pr} \\left\\{ B_m \\right\\} $$\n",
    "\n",
    "But\n",
    "\n",
    "$$ \\lim_{n \\rightarrow \\infty} \\sum_{m=1}^n \\text{Pr} \\left\\{ B_m \\right\\} = \\sum_{n=1}^\\infty \\text{Pr} \\left\\{ B_n \\right\\} $$\n",
    "\n",
    "which exists and is bound between 0 and 1 inclusive, since the right hand value the probability $\\text{Pr}\\left\\{ \\cup_{n=1}^\\infty A_n \\right\\}$.\n",
    "\n",
    "Therefore, by taking the limit to the result on finite sequences, we get\n",
    "\n",
    "$$  \\lim_{n \\rightarrow \\infty} \\text{Pr}\\left\\{ \\cup_{m=1}^n A_m \\right\\} = \\sum_{n=1}^\\infty \\text{Pr} \\left\\{ B_n \\right\\} = \\text{Pr}\\left\\{ \\cup_{n=1}^\\infty A_n \\right\\} $$\n",
    "\n",
    "which is the desired result."
   ]
  },
  {
   "cell_type": "markdown",
   "metadata": {},
   "source": [
    "**(f)**  De Morgan's equality states that\n",
    "\n",
    "$$ \\left(\\cap_{n=1}^\\infty A_n \\right)^c = \\cup_{n=1}^\\infty A_n^c $$\n",
    "\n",
    "By applying the result of (e) to the sequence of complements $A_1^c, A_2^c, \\dots$ we get:\n",
    "\n",
    "$$ \\lim_{n \\rightarrow \\infty} \\text{Pr}\\left\\{ \\cup_{m=1}^n A_m^c \\right\\} = \\text{Pr}\\left\\{ \\cup_{n=1}^\\infty A_n^c \\right\\} $$\n",
    "\n",
    "and using the fact that $\\text{Pr}\\left\\{ X \\right\\} + \\text{Pr}\\left\\{ X^c \\right\\} = 1$ we get\n",
    "\n",
    "$$ \\lim_{n \\rightarrow \\infty} 1 - \\text{Pr}\\left\\{ \\cap_{m=1}^n A_m \\right\\} = 1 - \\text{Pr}\\left\\{ \\cap_{n=1}^\\infty A_n \\right\\} $$\n",
    "\n",
    "from which the result follows,\n",
    "\n",
    "$$ \\lim_{n \\rightarrow \\infty} \\text{Pr}\\left\\{ \\cap_{m=1}^n A_m \\right\\} = \\text{Pr}\\left\\{ \\cap_{n=1}^\\infty A_n \\right\\} $$"
   ]
  },
  {
   "cell_type": "markdown",
   "metadata": {},
   "source": [
    "**Exercise 1.3**.  Find the probability that a five-card poker hand, chosen randomly from a 52-card deck, contains four aces.  That is, if all $52!$ arrangements of a deck of cards are equally likely, what is the probability that all four aces are in the first five cards of the deck."
   ]
  },
  {
   "cell_type": "markdown",
   "metadata": {},
   "source": [
    "**Solution**. There are $52 \\cdot 51 \\cdot 50 \\cdot 49 \\cdot 48$ ordered sequences for the first five cards of the deck.  Of those, the sequences containing four aces correspond to choosing the four aces in some order ($4 \\cdot 3 \\cdot 2 \\cdot 1$), then selecting a fifth card ($48$ choices) and inserting it somewhere alongside the first four cards ($5$ position choices).\n",
    "\n",
    "Therefore, the desired probability is\n",
    "\n",
    "$$ \\frac{(4 \\cdot 3 \\cdot 2 \\cdot 1) \\cdot 48 \\cdot 5}{52 \\cdot 51 \\cdot 50 \\cdot 49 \\cdot 48} = \\frac{1}{54145} $$"
   ]
  },
  {
   "cell_type": "code",
   "execution_count": null,
   "metadata": {},
   "outputs": [],
   "source": []
  }
 ],
 "metadata": {
  "kernelspec": {
   "display_name": "Python 3",
   "language": "python",
   "name": "python3"
  },
  "language_info": {
   "codemirror_mode": {
    "name": "ipython",
    "version": 3
   },
   "file_extension": ".py",
   "mimetype": "text/x-python",
   "name": "python",
   "nbconvert_exporter": "python",
   "pygments_lexer": "ipython3",
   "version": "3.7.3"
  }
 },
 "nbformat": 4,
 "nbformat_minor": 2
}
